use implicit generalization

isort.v
@@ -7,68 +7,67 @@ Import List.ListNotations.
 Open Scope list_scope.
 
 (* insert a number into a sorted list preserving the sortedness *)
-Fixpoint insert {A} {dto : DecTotalOrder A} (l : list A) (x : A) : list A :=
+Fixpoint insert {A} `{DecTotalOrder A} (l : list A) (x : A) : list A :=
   match l with
   | [] => [x]
   | h :: t => if leb_total_dec x h then x :: l else h :: insert t x
   end.
 
 (* insertion sort *)
-Fixpoint isort {A} {dto : DecTotalOrder A} (l : list A) : list A :=
+Fixpoint isort {A} `{DecTotalOrder A} (l : list A) : list A :=
   match l with
   | [] => []
   | h :: t => insert (isort t) h
   end.
 
-Lemma lem_insert_sorted_hlp {A} {dto : DecTotalOrder A} :
-  forall (l : list A) x y,
+Lemma lem_insert_sorted_hlp `{DecTotalOrder} :
+  forall l x y,
     leb x y -> Sorted (x :: l) -> Sorted (x :: insert l y).
 Proof.
   induction l; sauto q: on inv: Sorted ctrs: Sorted.
 Qed.
 
-Lemma lem_insert_sorted {A} {dto : DecTotalOrder A} (l : list A) (x : A) :
-  Sorted l -> Sorted (insert l x).
+Lemma lem_insert_sorted `{DecTotalOrder} :
+  forall l x, Sorted l -> Sorted (insert l x).
 Proof.
   destruct l; qauto use: lem_insert_sorted_hlp ctrs: Sorted.
 Qed.
 
-Lemma lem_isort_sorted {A} {dto : DecTotalOrder A} :
-  forall l : list A, Sorted (isort l).
+Lemma lem_isort_sorted `{DecTotalOrder} :
+  forall l, Sorted (isort l).
 Proof.
   induction l; sauto use: lem_insert_sorted.
 Qed.
 
-Lemma lem_insert_perm {A} {dto : DecTotalOrder A} :
-  forall (l : list A) x, Permutation (insert l x) (x :: l).
+Lemma lem_insert_perm `{DecTotalOrder} :
+  forall l x, Permutation (insert l x) (x :: l).
 Proof.
   induction l; sauto.
 Qed.
 
-Lemma lem_isort_perm {A} {dto : DecTotalOrder A} :
-  forall l : list A, Permutation (isort l) l.
+Lemma lem_isort_perm `{DecTotalOrder} :
+  forall l, Permutation (isort l) l.
 Proof.
   induction l; sauto use: lem_insert_perm.
 Qed.
 
 (* Boolean version *)
 
-Lemma lem_insert_sortedb_hlp {A} {dto : DecTotalOrder A} :
-  forall (l : list A) x y,
+Lemma lem_insert_sortedb_hlp `{DecTotalOrder} :
+  forall l x y,
     leb x y -> sortedb (x :: l) -> sortedb (x :: insert l y).
 Proof.
   induction l; hauto brefl: on.
 Qed.
 
-Lemma lem_insert_sortedb {A} {dto : DecTotalOrder A} :
-  forall (l : list A) x,
-    sortedb l -> sortedb (insert l x).
+Lemma lem_insert_sortedb `{DecTotalOrder} :
+  forall l x, sortedb l -> sortedb (insert l x).
 Proof.
   destruct l; hauto brefl: on use: lem_insert_sortedb_hlp.
 Qed.
 
-Lemma lem_isort_sortedb {A} {dto : DecTotalOrder A} :
-  forall l : list A, sortedb (isort l).
+Lemma lem_isort_sortedb `{DecTotalOrder} :
+  forall l, sortedb (isort l).
 Proof.
   induction l; sauto use: lem_insert_sortedb.
 Qed.
