sorted.v
@@ -4,13 +4,13 @@ Require Export Sorting.Permutation.
 Import List.ListNotations.
 Open Scope list_scope.
 
-Inductive Sorted {A} {dto : DecTotalOrder A} : list A -> Prop :=
+Inductive Sorted {A} `{DecTotalOrder A} : list A -> Prop :=
 | Sorted_0 : Sorted []
 | Sorted_1 : forall x, Sorted [x]
 | Sorted_2 : forall x y l, Sorted (y :: l) -> leb x y ->
                            Sorted (x :: y :: l).
 
-Lemma lem_sorted_tail {A} {dto : DecTotalOrder A} :
+Lemma lem_sorted_tail `{DecTotalOrder} :
   forall l x, Sorted (x :: l) -> Sorted l.
 Proof.
   sauto.
@@ -18,14 +18,14 @@ Qed.
 
 (*********************************************************************)
 
-Fixpoint sortedb {A} {dto : DecTotalOrder A} (l : list A) : bool :=
+Fixpoint sortedb {A} `{DecTotalOrder A} (l : list A) : bool :=
   match l with
   | [] => true
   | [x] => true
   | x :: (y :: l') as t => leb x y && sortedb t
   end.
 
-Lemma lem_sortedb_iff_sorted {A} {dto : DecTotalOrder A} :
+Lemma lem_sortedb_iff_sorted `{DecTotalOrder} :
   forall l : list A, sortedb l <-> Sorted l.
 Proof.
   induction l; sauto brefl: on inv: Sorted.
@@ -33,50 +33,50 @@ Qed.
 
 (*********************************************************************)
 
-Definition LeLst {A} {dto : DecTotalOrder A} (x : A) :=
+Definition LeLst `{DecTotalOrder} x :=
   List.Forall (leb x).
 
-Lemma lem_lelst_nil {A} {dto : DecTotalOrder A} : forall x, LeLst x [].
+Lemma lem_lelst_nil `{DecTotalOrder} : forall x, LeLst x [].
 Proof.
   sauto.
 Qed.
 
-Lemma lem_lelst_cons {A} {dto : DecTotalOrder A} :
+Lemma lem_lelst_cons `{DecTotalOrder} :
   forall x y l, LeLst x l -> leb x y -> LeLst x (y :: l).
 Proof.
   sauto.
 Qed.
 
-Hint Resolve lem_lelst_nil lem_lelst_cons : lelst.
+Global Hint Resolve lem_lelst_nil lem_lelst_cons : lelst.
 
-Lemma lem_lelst_trans {A} {dto : DecTotalOrder A} :
+Lemma lem_lelst_trans `{DecTotalOrder} :
   forall l x y, LeLst y l -> leb x y -> LeLst x l.
 Proof.
   induction 1; sauto.
 Qed.
 
-Lemma lem_lelst_perm {A} {dto : DecTotalOrder A} :
+Lemma lem_lelst_perm `{DecTotalOrder} :
   forall l1 l2 x, Permutation l1 l2 -> LeLst x l1 -> LeLst x l2.
 Proof.
   induction 1; sauto lq: on.
 Qed.
 
-Lemma lem_lelst_perm_rev {A} {dto : DecTotalOrder A} :
+Lemma lem_lelst_perm_rev `{DecTotalOrder} :
   forall l1 l2 x, Permutation l1 l2 -> LeLst x l2 -> LeLst x l1.
 Proof.
   induction 1; sauto lq: on.
 Qed.
 
-Lemma lem_lelst_app {A} {dto : DecTotalOrder A} :
+Lemma lem_lelst_app `{DecTotalOrder} :
   forall l1 l2 x, LeLst x l1 -> LeLst x l2 -> LeLst x (l1 ++ l2).
 Proof.
   induction 1; sauto lq: on.
 Qed.
 
-Hint Resolve lem_lelst_trans lem_lelst_perm lem_lelst_perm_rev
-     lem_lelst_app : lelst.
+Global Hint Resolve lem_lelst_trans lem_lelst_perm lem_lelst_perm_rev
+       lem_lelst_app : lelst.
 
-Lemma lem_lelst_sorted {A} {dto : DecTotalOrder A} :
+Lemma lem_lelst_sorted `{DecTotalOrder} :
   forall l x, Sorted (x :: l) <-> LeLst x l /\ Sorted l.
 Proof.
   induction l; sauto l: on use: lem_lelst_trans
@@ -85,45 +85,45 @@ Qed.
 
 (*********************************************************************)
 
-Definition GeLst {A} {dto : DecTotalOrder A} (x : A) (l : list A) :=
+Definition GeLst `{DecTotalOrder} x l :=
   List.Forall (fun y => leb y x) l.
 
-Lemma lem_gelst_nil {A} {dto : DecTotalOrder A} : forall x, GeLst x [].
+Lemma lem_gelst_nil `{DecTotalOrder} : forall x, GeLst x [].
 Proof.
   sauto.
 Qed.
 
-Lemma lem_gelst_cons {A} {dto : DecTotalOrder A} :
+Lemma lem_gelst_cons `{DecTotalOrder} :
   forall x y l, GeLst x l -> leb y x -> GeLst x (y :: l).
 Proof.
   sauto.
 Qed.
 
-Hint Resolve lem_gelst_nil lem_gelst_cons : gelst.
+Global Hint Resolve lem_gelst_nil lem_gelst_cons : gelst.
 
-Lemma lem_gelst_trans {A} {dto : DecTotalOrder A} :
+Lemma lem_gelst_trans `{DecTotalOrder} :
   forall l x y, GeLst y l -> leb y x -> GeLst x l.
 Proof.
   induction 1; sauto.
 Qed.
 
-Lemma lem_gelst_perm {A} {dto : DecTotalOrder A} :
+Lemma lem_gelst_perm `{DecTotalOrder} :
   forall x l1 l2, Permutation l1 l2 -> GeLst x l1 -> GeLst x l2.
 Proof.
   induction 1; sauto lq: on.
 Qed.
 
-Lemma lem_gelst_perm_rev {A} {dto : DecTotalOrder A} :
+Lemma lem_gelst_perm_rev `{DecTotalOrder} :
   forall l1 l2 x, Permutation l1 l2 -> GeLst x l2 -> GeLst x l1.
 Proof.
   induction 1; sauto lq: on.
 Qed.
 
-Lemma lem_gelst_app {A} {dto : DecTotalOrder A} :
+Lemma lem_gelst_app `{DecTotalOrder} :
   forall l1 l2 x, GeLst x l1 -> GeLst x l2 -> GeLst x (l1 ++ l2).
 Proof.
   induction 1; sauto lq: on.
 Qed.
 
-Hint Resolve lem_gelst_trans lem_gelst_perm lem_gelst_perm_rev
+Global Hint Resolve lem_gelst_trans lem_gelst_perm lem_gelst_perm_rev
      lem_gelst_app : gelst.
